Working on Theorem 6', Theorem 7' and finished 8 and 8'.

kacc_undec.v
@@ -5,14 +5,17 @@ Require Import Coq.Setoids.Setoid.
 Require Import Undecidability.MinskyMachines.MM2.
 Require Import Coq.Sets.Ensembles.
 Require Import Coq.Sets.Finite_sets.
+(* From Coq Require Import Lia. *)
 
 From Coq Require Import List. Import ListNotations.
 From Coq Require Import Bool.
 
-(* Require Import List Relations.Relation_Operators. *)
+Set Implicit Arguments.
+Unset Strict Implicit.
+Unset Printing Implicit Defensive.
 
-Check mm2_step.
-Print mm2_step.
+
+(* Require Import List Relations.Relation_Operators. *)
 
 (* Print mm2_instr_at.
 #[local] Set Implicit Arguments.
@@ -23,10 +26,10 @@ Check (clos_refl_trans _ (mm2_step _)). *)
 (* ------- Commuting Relations ------- *)
 (* ------- ------- *)
 
-Definition commuting_relation X (R : Relation_Definitions.relation X) :=
+(* Definition commuting_relation X (R : Relation_Definitions.relation X) :=
   Reflexive R /\ Symmetric R.
 
-Definition commute X R (H : commuting_relation X R) (x y : X) := R x y.
+Definition commute X R (H : commuting_relation R) (x y : X) := R x y.
 
 Definition commutable X R := commuting_relation X R.
 
@@ -34,7 +37,7 @@ Definition discrete X R (H : commuting_relation X R) (x y : X) :=
   R x y <-> x = y. (* QUEST: what kind of equality is meant here? *)
 
 Definition commutative X R (H : commuting_relation X R) :=
-  ∀ (x y : X), commute X R H x y.
+  ∀ (x y : X), commute X R H x y. *)
 
 (* ------- ------- *)
 (* ------- string over set ------- *)
@@ -68,7 +71,7 @@ Arguments K_Dot {T}.
 Arguments K_Star {T}.
 
 Declare Scope ka_scope.
-Delimit Scope ka_scope with T.
+Delimit Scope ka_scope with ka.
 Bind Scope ka_scope with ka_term.
 
 Fixpoint ka_power {T} (x : ka_term T) (n : nat) :=
@@ -89,7 +92,7 @@ Definition lr_term {T} (x : T) := K_Dot (L x) (R x).
 (* TODO: come back to scoping here *)
 Notation "'lr' x" := (lr_term x) (at level 30, no associativity): ka_scope.
 
-Reserved Notation "e1 ≐ e2" (at level 80, no associativity).
+Reserved Notation "e1 ≡ e2" (at level 80, no associativity).
 
 Inductive ka_eq {T : Type} : ka_term T -> ka_term T -> Prop :=
   | Ka_refl : Reflexive (@ka_eq T)
@@ -101,24 +104,26 @@ Inductive ka_eq {T : Type} : ka_term T -> ka_term T -> Prop :=
   | Ka_Star : Proper ((@ka_eq T) ==> (@ka_eq T)) K_Star
 
   (* including the following to allow for commuting terms *)
-  | LR_Com x y : (L x)⋅(R y) ≐ (R y)⋅(L x)
+  | LR_Com x y : (L x)⋅(R y) ≡ (R y)⋅(L x)
 
-  | Dot_Id1 t : t ⋅ 1 ≐ t
-  | Dot_Id2 t : 1 ⋅ t ≐ t
-  | Dot_Z1  t : t ⋅ 0 ≐ 0
-  | Dot_Z2  t : 0 ⋅ t ≐ 0
-  | Dot_Assoc x y z : x ⋅ (y ⋅ z) ≐ (x ⋅ y) ⋅ z
+  | Dot_Id1 t : t ⋅ 1 ≡ t
+  | Dot_Id2 t : 1 ⋅ t ≡ t
+  | Dot_Z1  t : t ⋅ 0 ≡ 0
+  | Dot_Z2  t : 0 ⋅ t ≡ 0
+  | Dot_Assoc x y z : x ⋅ (y ⋅ z) ≡ (x ⋅ y) ⋅ z
 
-  | Plus_Id t : 0 + t ≐ t
-  | Plus_Com (x y : ka_term T) : x + y ≐ y + x
-  | Plus_Assoc x y z : x + (y + z) ≐ (x + y) + z
-  | Plus_Idemp x : x + x ≐ x
+  | Plus_Id t : 0 + t ≡ t
+  | Plus_Com (x y : ka_term T) : x + y ≡ y + x
+  | Plus_Assoc x y z : x + (y + z) ≡ (x + y) + z
+  | Plus_Idemp x : x + x ≡ x
 
-  | Dist_L x y z : x ⋅ (y + z) ≐ x⋅y + x⋅z
-  | Dist_R x y z : (x + y) ⋅ z ≐ x⋅z + y⋅z
+  | Dist_L x y z : x ⋅ (y + z) ≡ x⋅y + x⋅z
+  | Dist_R x y z : (x + y) ⋅ z ≡ x⋅z + y⋅z
 
-  | Star t : t✶ ≐ 1 + (t ⋅ (t✶))
-  where "e1 ≐ e2" := (ka_eq e1 e2) : ka_scope.
+  | Star t : t✶ ≡ 1 + (t ⋅ (t✶))
+  where "e1 ≡ e2" := (ka_eq e1 e2).
+
+Notation "x ≢ y" := (not (ka_eq x y)) (at level 80, no associativity).
 
 Global Existing Instance Ka_refl.
 Global Existing Instance Ka_sym.
@@ -129,10 +134,25 @@ Global Existing Instance Ka_Star.
 
 Add Parametric Relation T : (ka_term T) ka_eq as ka_eq.
 
-Definition ka_leq {T} (x y : ka_term T) : Prop := ((y + x) ≐ y)%T. (* this is a typo in the paper? *)
+Lemma Plus_Id' : ∀ T (t : ka_term T), t + 0 ≡ t.
+Proof.
+  intros T t.
+  rewrite Plus_Com; rewrite Plus_Id.
+  reflexivity.
+Qed.
+
+Lemma ka_neq_sym : ∀ T (x y : ka_term T), x ≢ y <-> y ≢ x.
+Proof.
+  intros T x y; split; intros H G; symmetry in G; apply H in G; assumption.
+Qed.
+
+(* QUEST: How to declare this to work with symmetry tactic? *)
+Hint Resolve ka_neq_sym : core.
+(* Global Existing Instance ka_neq_sym. *)
+
+Definition ka_leq {T} (x y : ka_term T) : Prop := ((y + x) ≡ y)%ka.
 Notation "x ≤ y" := (ka_leq x y) : ka_scope.
 
-(* Global Instance  *)
 
 (* ------- ------- *)
 (* ------- Interpreting MM instructions as terms ------- *)
@@ -155,93 +175,51 @@ Qed.
 
 Hint Resolve leq_reflex : core.
 Variable T : Type.
-Implicit Types (e : ka_term T) (x y z : T).
+
+Lemma leq_trans : ∀ (t1 t2 t3 : ka_term T), t1 ≤ t2 -> t2 ≤ t3 -> t1 ≤ t3.
+Proof.
+  intros.
+  unfold ka_leq in *.
+  rewrite - H0.
+  rewrite - H.
+  rewrite Plus_Assoc.
+  rewrite - Plus_Assoc.
+  rewrite Plus_Idemp.
+  reflexivity.
+Qed.
 
 Global Instance leq_proper :
   Proper (ka_eq ==> ka_eq ==> iff) (@ka_leq T).
 Proof.
   rewrite /ka_leq => e1 e2 e12 e3 e4 e34.
   split.
-  - intros. rewrite <- e34. rewrite <- e12. assumption.
+  - intros. rewrite - e34. rewrite - e12. assumption.
   - intros. rewrite e12. rewrite e34. assumption.
 Qed.
 
-Lemma star_expand : forall (t : ka_term T), t✶ ≐ 1 + t⋅t✶.
+Lemma star_expand : forall (t : ka_term T), t✶ ≡ 1 + t⋅t✶.
 Proof. intros. apply Star. Qed.
 
 Lemma star_leq : forall (t : ka_term T), 1 + t⋅t✶ ≤ t✶.
 Proof.
   intros.
-  rewrite <- star_expand.
+  rewrite - star_expand.
   apply leq_reflex.
 Qed.
 
-Lemma leq_antisym : forall (x y : ka_term T), x ≤ y -> y ≤ x -> x ≐ y.
+Lemma leq_antisym : forall (x y : ka_term T), x ≤ y -> y ≤ x -> x ≡ y.
 Proof.
   intros.
   unfold ka_leq in H, H0.
-  rewrite <- H. rewrite Plus_Com. symmetry. assumption.
+  rewrite - H. rewrite Plus_Com. symmetry. assumption.
 Qed.
 
-(* Lemma not_L_eq_0 : ∀ a : T, not (L a ≐ 0).
-Proof.
-  unfold not. intros.
-  inversion
-Admitted.
+Definition build_term (side : T -> ka_term T) := fold_right (λ (n : T) t, side n ⋅ t).
 
-Lemma dot_eq_zero : ∀ e1 e2,  e1 ⋅ e2 ≐ 0 -> (e1 ≐ 0) \/ (e2 ≐ 0).
-Proof.
-  intros.
-  induction e1.
-  - left; reflexivity.
-  - rewrite Dot_Id2 in H. right; assumption.
-  - right. destruct e2.
-    + reflexivity.
-    + rewrite Dot_Id1 in H. apply not_L_eq_0 in H. contradiction.
-    + inversion H; subst.
-  destruct (L t) eqn:eqlt; try (inversion eqlt); subst.
-    + inversion eqlt.
-    +
-  inversion H.
-
-Lemma plus_elim : ∀ (ex1 ex2 : ka_term T) (side : T -> ka_term T) a, (side = L) \/ (side = R) -> side a ⋅ ex1 ≐ side a ⋅ ex2 -> ex1 ≐ ex2.
-Proof.
-  intros.
-  destruct H as [H1 | H2]; subst.
-  - remember (L a0) as l.
-    induction ex1.
-    + rewrite Dot_Z1 in H0. subst.
-    inversion H0; subst; try reflexivity.
-    +
-   induction ex1.
-    + inversion H0; subst; try reflexivity.
-      *
-   remember (L a0) as l.
-    induction ex1.
-    + subst. induction ex2; try reflexivity.
-      * rewrite Dot_Z1 in H0. rewrite Dot_Id1 in H0. inversion H0; subst.
-  induction H. inversion H0; subst; try reflexivity.
-    +
-  -
-  induction ex1.
-  - rewrite Dot_Z1 in H. inversion H.
-    +
-  inversion H.
-  - reflexivity.
-  -
-  induction ex1.
-  - inversion H; try reflexivity. *)
-
-Definition string_to_ka_term side ls :=
-  List.fold_left (* TODO: use fold_right*)
-    (* (ka_term T) T *)
-    (λ (t : ka_term T) (new : T), t⋅(side new))
-    ls 1.
-
-Print List.fold_left.
-Print List.fold_right.
-
-Definition step exp s s' := (string_to_ka_term L s) ⋅ (string_to_ka_term R s') ≤ exp.
+Definition string_to_ka_term ls :=
+  match ls with (l1, l2) =>
+    (build_term L 1 l1)⋅(build_term R 1 l2)
+  end.
 
 Definition interp (n : nat) (P : list mm2_instr) :=
   match nth n P mm2_inc_a with
@@ -253,23 +231,59 @@ Definition interp (n : nat) (P : list mm2_instr) :=
                     + (lr a)✶ ⋅ L b ⋅ (lr b)✶ ⋅ (R (Q_M (S n)))
   end.
 
+Definition interp_single (n : nat) (instr : mm2_instr) :=
+  match instr with
+  | mm2_inc_a =>    R a ⋅ (lr a)✶ ⋅ (lr b)✶ ⋅ R (Q_M (S n))
+  | mm2_inc_b =>    (lr a)✶ ⋅ R b ⋅ (lr b)✶  ⋅ R (Q_M (S n))
+  | mm2_dec_a n' => (lr b)✶ ⋅ (R (Q_M n'))
+                    + L a ⋅ (lr a)✶ ⋅ (lr b)✶ ⋅ (R (Q_M (S n)))
+  | mm2_dec_b n' => (lr a)✶ ⋅ (R (Q_M n'))
+                    + (lr a)✶ ⋅ L b ⋅ (lr b)✶ ⋅ (R (Q_M (S n)))
+  end.
+
 Definition pair_append (s1 s2 : list T * list T) :=
   match s1, s2 with
   | (s1l, s1r), (s2l, s2r) => (s1l ++ s2l, s1r ++ s2r)
   end.
 
-Check ka_power.
+Lemma pair_append_eq_nil : ∀ s s',
+  pair_append s s' = ([], []) -> s = ([], []) ∧ s' = ([], []).
+Proof.
+  intros.
+  destruct s, s'.
+  simpl in H; injection H;
+  intros G K; clear H.
+  apply app_eq_nil in G as [G1 G2], K as [K1 K2];
+  subst;
+  auto.
+Qed.
 
-(* Fixpoint lang_interp_power (term : ka_term T) (n : nat) {struct term} : (list T * list T) -> Prop :=
-  match n with
-  | 0%nat => λ s, s = ([], [])
-  | S n' => λ s, ∃ s1 s2, s = pair_append s1 s2 /\ lang_interp term s1 /\ lang_interp_power term n' s2
-  end *)
+(* used *)
+Lemma pair_append_id_r : ∀ s, pair_append s ([], []) = s.
+Proof.
+  intros. unfold pair_append.
+  destruct s.
+  repeat (rewrite List.app_nil_r).
+  reflexivity.
+Qed.
 
-Print ka_power.
+(* used *)
+Lemma pair_append_id_l : ∀ s, pair_append ([], []) s = s.
+Proof.
+  intros. unfold pair_append.
+  destruct s.
+  repeat (rewrite List.app_nil_l).
+  reflexivity.
+Qed.
 
-Definition pair_length (s : list T * list T) :=
-  match s with (l1, l2) => Nat.add (List.length l1) (List.length l2) end.
+(* used *)
+Lemma pair_append_assoc : ∀ s1 s2 s3,
+  pair_append s1 (pair_append s2 s3) = pair_append (pair_append s1 s2) s3.
+Proof.
+  intros.
+  destruct s1, s2, s3.
+  simpl. repeat (rewrite List.app_assoc); reflexivity.
+Qed.
 
 Definition ka_pred_zero (s : list T * list T) := False.
 
@@ -301,106 +315,32 @@ Fixpoint lang_interp term :=
   | e✶ => ka_pred_star (lang_interp e)
   end.
 
-(* Fixpoint ka_power_pred e n s {measure (pair_length s)}:=
-  match n with
-  | 0%nat => s = ([], [])
-  | S n => ∃ s1 s2, s = pair_append s1 s2 /\ lang_interp e s1 /\ ka_power_pred e n s2
-  end
-
-with lang_interp term s {measure (pair_length s)} :=
-  match term with
-  | 0 => False
-  | 1 => s = ([], [])
-  | L e => s = ([e], [])
-  | R e => s = ([], [e])
-  | e1 + e2 => lang_interp e1 s \/ lang_interp e2 s
-  | e1 ⋅ e2 => ∃ s1 s2, s = pair_append s1 s2 /\ lang_interp e1 s1 /\ lang_interp e2 s2
-  (* | e✶ => λ s, ∃ (n : nat), lang_interp_power e n s *)
-  | e✶ => ∃ n, ka_power_pred e n s
-  (* λ s, True *)
-  (* λ s, ∃ n, ka_power_pred e n s *)
-  (* λ s, ∃ n, lang_interp (ka_power e n) s *)
-  (* s = ([], []) \/ ∃ s1 s2, s = pair_append s1 s2 /\ lang_interp e s1 /\ lang_interp e(* ✶ *) s2 *)
-  end. *)
-
-Check lang_interp.
-
-(* Lemma l_i_plus : ∀ (x x' : ka_term T) s,
-  lang_interp (x + x') s <->
-    lang_interp x s \/ lang_interp x' s.
-Proof.
-  intros; unfold lang_interp; reflexivity.
-Qed. *)
-
-(* Lemma l_i_dot : ∀ (x x' : ka_term T) s,
-  lang_interp (x ⋅ x') s <->
-    ∃ s1 s2, s = pair_append s1 s2 /\ lang_interp x s1 /\ lang_interp x' s2.
-Proof.
-  intros; unfold lang_interp; reflexivity.
-Qed. *)
-
-(* Lemma l_i_star : ∀ (x : ka_term T) s,
-  lang_interp (x✶) s <-> s = ([], []) \/ ∃ s1 s2, s = pair_append s1 s2 /\ lang_interp x s1 /\ lang_interp x s2.
-Proof.
-  intros; unfold lang_interp; reflexivity.
-Qed. *)
-
-Lemma pair_append_id_r : ∀ s, pair_append s ([], []) = s.
-Proof.
-  intros. unfold pair_append.
-  destruct s.
-  repeat (rewrite List.app_nil_r).
-  reflexivity.
-Qed.
-
-Lemma pair_append_id_l : ∀ s, pair_append ([], []) s = s.
-Proof.
-  intros. unfold pair_append.
-  destruct s.
-  repeat (rewrite List.app_nil_l).
-  reflexivity.
-Qed.
-
-Lemma pair_append_assoc : ∀ s1 s2 s3, pair_append s1 (pair_append s2 s3) = pair_append (pair_append s1 s2) s3.
-Proof.
-  intros.
-  destruct s1, s2, s3.
-  simpl. repeat (rewrite List.app_assoc); reflexivity.
-Qed.
-
+(* used *)
 Lemma l_i_dot_1_r : ∀ (x : ka_term T) s, lang_interp (x ⋅ 1) s <-> lang_interp x s.
 Proof.
-  split; intros.
-  - simpl in H. destruct H as [s1 [s2 [H1 [H2 H3]]]].
-    subst. rewrite pair_append_id_r. assumption.
-  - simpl.
-    exists s, ([], []); repeat split.
-    + symmetry. apply pair_append_id_r.
-    + assumption.
+  split; intros; simpl in *.
+  - destruct H as [s1 [s2 [H1 [H2 H3]]]];
+    unfold ka_pred_unit in H3; subst;
+    rewrite pair_append_id_r; assumption.
+  - simpl; exists s, ([], []); repeat split;
+    [symmetry; apply pair_append_id_r | assumption].
 Qed.
 
+(* used *)
 Lemma l_i_dot_1_l : ∀ (x : ka_term T) s, lang_interp (1 ⋅ x) s <-> lang_interp x s.
 Proof.
-  split; intros.
-  - simpl in H. destruct H as [s1 [s2 [H1 [H2 H3]]]].
-    subst. rewrite pair_append_id_l. assumption.
-  - simpl.
-    exists ([], []), s; repeat split.
-    + symmetry. apply pair_append_id_l.
-    + assumption.
+  split; intros; simpl in *.
+  - destruct H as [s1 [s2 [H1 [H2 H3]]]];
+    unfold ka_pred_unit in H2; subst;
+    rewrite pair_append_id_l; assumption.
+  - exists ([], []), s; repeat split;
+    [symmetry; apply pair_append_id_l | assumption].
 Qed.
 
-(* Theorem term_lang_equiv : ∀ s t, string_to_ka_term L s ≤ t <-> lang_interp t (s, []).
+(* QUEST: do we need bidirectionality here? I don't think this holds...but wanted to check *)
+Theorem l_i_equality : ∀ t1 t2, t1 ≡ t2 -> ∀ s, lang_interp t1 s <-> lang_interp t2 s.
 Proof.
-  split; intros.
-  induction t.
-  - compute in H.
-  simpl. *)
-
-Theorem l_i_equality : ∀ t1 t2, t1 ≐ t2 -> ∀ s, lang_interp t1 s <-> lang_interp t2 s.
-Proof.
-  intros.
-  generalize dependent s.
+  intros t1 t2 H.
   induction H.
   - reflexivity.
   - intros. symmetry. apply IHka_eq.
@@ -408,131 +348,954 @@ Proof.
   - simpl; split; intros; destruct H1 as [H1 | H1].
     + rewrite IHka_eq1 in H1; left; assumption.
     + rewrite IHka_eq2 in H1; right; assumption.
-    + rewrite <- IHka_eq1 in H1; left; assumption.
-    + rewrite <- IHka_eq2 in H1; right; assumption.
+    + rewrite - IHka_eq1 in H1; left; assumption.
+    + rewrite - IHka_eq2 in H1; right; assumption.
   - simpl; split; intros;
     destruct H1 as [s1 [s2 [G1 [G2 G3]]]]; exists s1, s2;
     repeat split; try assumption.
     + rewrite IHka_eq1 in G2; assumption.
     + rewrite IHka_eq2 in G3; assumption.
-    + rewrite <- IHka_eq1 in G2; assumption.
-    + rewrite <- IHka_eq2 in G3; assumption.
-  - simpl; split; intros;
-    destruct H0 as [Hem | [s1 [s2 [H1 [H2 H3]]]]];
-    try (left; assumption).
-    + right; exists s1, s2; repeat split; try assumption.
-      * rewrite IHka_eq in H2; assumption.
-      * rewrite IHka_eq in H3; assumption.
-    + right; exists s1, s2; repeat split; try assumption.
-      * rewrite <- IHka_eq in H2; assumption.
-      * rewrite <- IHka_eq in H3; assumption.
-  - intros. unfold lang_interp in *.
+    + rewrite - IHka_eq1 in G2; assumption.
+    + rewrite - IHka_eq2 in G3; assumption.
+  - simpl; split; intros G;
+    unfold ka_pred_star, ka_pred_power, ka_pred_unit, ka_pred_mul in *;
+    destruct G as [n G];
+    exists n; generalize dependent s; induction n;
+    simpl in *; intros; try assumption;
+    destruct G as [s1 [s2 [Hs1s2 [HLI1 Hiter]]]];
+    exists s1, s2; repeat split; try assumption;
+    try (apply IHn; assumption);
+    [rewrite - IHka_eq; assumption | rewrite IHka_eq; assumption].
+  - intros; unfold lang_interp, ka_pred_mul, ka_pred_left, ka_pred_right in *;
     split; intros; destruct H as [s1 [s2 [H1 [H2 H3]]]];
     exists s2, s1; repeat split; try assumption; subst; reflexivity.
   - intros; rewrite l_i_dot_1_r; reflexivity.
   - intros; rewrite l_i_dot_1_l; reflexivity.
   - split; intros; simpl in *;
+    unfold ka_pred_mul, ka_pred_zero in *;
     [destruct H as [_ [_ [_ [_ H]]]]; assumption | contradiction].
   - split; intros; simpl in *;
+    unfold ka_pred_mul, ka_pred_zero in *;
     [destruct H as [_ [_ [_ [H _]]]]; assumption | contradiction].
-  - split; intros; simpl in *.
+  - split; intros; simpl in *;
+    unfold ka_pred_mul in *.
     + destruct H as [s1 [s2 [Hs1s2 [HLI1 [s3 [s4 [Hs3s4 [HLI3 HLI4]]]]]]]].
-      exists (pair_append s1 s3), s4; repeat split.
-      * rewrite <- pair_append_assoc. rewrite <- Hs3s4; assumption.
+      exists (pair_append s1 s3), s4; repeat split; try assumption.
+      * rewrite - pair_append_assoc. rewrite - Hs3s4; assumption.
       * exists s1, s3; repeat split; assumption.
-      * assumption.
     + destruct H as [s1 [s2 [Hs1s2 [[s3 [s4 [Hs3s4 [HLI3 HLI4]]]] HLI2]]]].
-      exists s3, (pair_append s4 s2); repeat split.
-      * rewrite pair_append_assoc; rewrite <- Hs3s4; assumption.
-      * assumption.
+      exists s3, (pair_append s4 s2); repeat split; try assumption.
+      * rewrite pair_append_assoc; rewrite - Hs3s4; assumption.
       * exists s4, s2; repeat split; assumption.
   - simpl; split; intros; [destruct H; [contradiction | assumption] | right; assumption].
-  - simpl; intros; rewrite or_comm; reflexivity.
-  - simpl; intros; rewrite or_assoc; reflexivity.
-  - simpl; split; intros.
-    + destruct H; assumption.
-    + left; assumption.
-  - simpl; split; intros.
-    + destruct H as [s1 [s2 [HS1s2 [HLI1 [HLI2 | HLI3]]]]].
-      * left;  exists s1, s2; repeat split; assumption.
-      * right; exists s1, s2; repeat split; assumption.
-    + destruct H as [[s1 [s2 [Hs1s2 [HLI1 HLI2]]]] | [s1 [s2 [Hs1s2 [HLI1 HLI2]]]]].
-      * exists s1, s2; repeat split; try assumption; left; assumption.
-      * exists s1, s2; repeat split; try assumption; right; assumption.
-  - simpl; split; intros.
-    + destruct H as [s1 [s2 [Hs1s2 [[HS1|HS1] HS2]]]].
-      * left;  exists s1, s2; repeat split; assumption.
-      * right; exists s1, s2; repeat split; assumption.
-    + destruct H as [[s1 [s2 [Hs1s2 [HLI1 HLI2]]]] | [s1 [s2 [Hs1s2 [HLI1 HLI2]]]]].
-      * exists s1, s2; repeat split; try assumption; left; assumption.
-      * exists s1, s2; repeat split; try assumption; right; assumption.
-  - simpl. split; intros.
-    + destruct H.
+  - simpl; intros; unfold ka_pred_add in *; rewrite or_comm; reflexivity.
+  - simpl; intros; unfold ka_pred_add in *; rewrite or_assoc; reflexivity.
+  - simpl; split; intros; unfold ka_pred_add in *;
+    [destruct H; assumption | left; assumption].
+  - simpl; split; intros; unfold ka_pred_add, ka_pred_mul in *.
+    + destruct H as [s1 [s2 [HS1s2 [HLI1 [HLI2 | HLI3]]]]];
+      [left | right]; exists s1, s2; repeat split; assumption.
+    + destruct H as [[s1 [s2 [Hs1s2 [HLI1 HLI2]]]] | [s1 [s2 [Hs1s2 [HLI1 HLI2]]]]];
+      exists s1, s2; repeat split; try assumption; [left | right]; assumption.
+  - simpl; split; intros; unfold ka_pred_add, ka_pred_mul in *.
+    + destruct H as [s1 [s2 [Hs1s2 [[HS1|HS1] HS2]]]];
+      [left | right]; exists s1, s2; repeat split; assumption.
+    + destruct H as [[s1 [s2 [Hs1s2 [HLI1 HLI2]]]] | [s1 [s2 [Hs1s2 [HLI1 HLI2]]]]];
+      exists s1, s2; repeat split; try assumption; [left | right]; assumption.
+  - simpl; split; intros; unfold ka_pred_star in *.
+    + destruct H as [n H].
+      unfold ka_pred_add, ka_pred_power in *.
+      destruct n; simpl in H.
       * left; assumption.
-      * right; destruct H as [s1 [s2 [Hs1s2 [HLI1 HLI2]]]].
-        exists s1, (pair_append s2 ([], [])); repeat split.
-        -- rewrite pair_append_id_r; assumption.
-        -- assumption.
-        -- right.
-        exists s1, s2; repeat split; try assumption.
-        right. exists s2, ([], []); repeat split.
-        -- symmetry; apply pair_append_id_r.
-        -- assumption.
-        --
-   simpl; split; intros.
-    + destruct H as [HS | [s1 [s2 [Hs1s2 [HLI1 HLI2]]]]].
-      * left; assumption.
-      * right. exists s1, s2. repeat split; try assumption.
-       right; exists s1, s2; repeat split; try assumption.
+      * unfold ka_pred_mul in H;
+        destruct H as [s1 [s2 [Hs1s2 [HS1 Hpow]]]];
+        unfold ka_pred_add, ka_pred_mul, ka_pred_star; right;
+        exists s1, s2; repeat split; try assumption;
+        exists n; assumption.
+    + unfold ka_pred_add in H; destruct H as [H | H].
+      * exists 0%nat; simpl; assumption.
+      * unfold ka_pred_power, ka_pred_mul in *;
+        destruct H as [s1 [s2 [Hs1s2 [HLI1 [n HPow]]]]];
+        subst; exists (S n); simpl;
+        exists s1, s2; repeat split; assumption.
+Qed.
+
+Global Instance lang_interp_proper : Proper (ka_eq ==> eq ==> iff) lang_interp.
+Proof.
+  intros t1 t2 et1t2 s1 s2 es1s2.
+  rewrite es1s2.
+  apply l_i_equality.
+  assumption.
+Qed.
+
+(* used *)
+Lemma leq_leq_dot : ∀ (x1 x2 y1 y2 : ka_term T), x1 ≤ y1 -> x2 ≤ y2 -> x1⋅x2 ≤ y1⋅y2.
+Proof.
+  intros x1 x2 y1 y2 H G.
+  unfold ka_leq in H, G.
+  unfold ka_leq.
+  rewrite - H; rewrite - G.
+  rewrite Dist_L; repeat (rewrite Dist_R).
+  rewrite Plus_Assoc; rewrite - Plus_Assoc.
+  rewrite Plus_Idemp.
+  reflexivity.
+Qed.
+
+(* used *)
+Lemma leq_plus : ∀ (x1 x2 : ka_term T), x1 ≤ x1 + x2.
+Proof.
+  intros.
+  unfold ka_leq.
+  rewrite Plus_Com;
+  rewrite Plus_Assoc;
+  rewrite Plus_Idemp.
+  reflexivity.
+Qed.
+
+(* used *)
+Lemma one_leq_star : ∀ (t : ka_term T), 1 ≤ t ✶.
+Proof.
+  intros.
+  rewrite Star.
+  apply leq_plus.
+Qed.
+
+(* used *)
+Lemma li_term_to_string_true : ∀ s, lang_interp (string_to_ka_term s) s.
+Proof.
+  intros.
+  destruct s as (sl, sr).
+  simpl.
+  exists (sl, []), ([], sr).
+  repeat split.
+  - simpl. rewrite app_nil_r; reflexivity.
+  - induction sl as [| e1 sl' IHsl'].
+    + reflexivity.
+    + simpl. unfold ka_pred_mul.
+      exists ([e1], []), (sl', []).
+      repeat split. assumption.
+  - induction sr as [| e1 sr' IHsr'].
+    + reflexivity.
+    + simpl. unfold ka_pred_mul.
+      exists ([], [e1]), ([], sr').
+      repeat split. assumption.
+Qed.
+
+(* unused *)
+Lemma build_term__pull_out_base : ∀ s (side : T -> ka_term T) (t : ka_term T),
+  side = R ∨ side = L -> build_term side t s
+    ≡ (build_term side 1 s) ⋅ t.
+Proof.
+  intros. destruct H as [H | H];
+  generalize dependent t;
+  try (induction s; intros; simpl; [
+    rewrite Dot_Id2; reflexivity
+  | rewrite IHs; rewrite Dot_Assoc; reflexivity
+  ]).
+Qed.
+
+(* used *)
+Lemma build_term__commutes : ∀ s t side1 side2,
+  (side1 = L ∧ side2 = R) ∨ (side1 = R ∧ side2 = L) ->
+  (build_term side1 1 s) ⋅ side2 t
+    ≡ side2 t ⋅ (build_term side1 1 s).
+Proof.
+  intros.
+  destruct H as [H | H]; destruct H as [H1 H2]; subst;
+  try (induction s as [|c s IHs]; simpl; [
+      rewrite Dot_Id2; rewrite Dot_Id1; reflexivity
+    | rewrite - Dot_Assoc; rewrite IHs;
+      repeat (rewrite Dot_Assoc); rewrite LR_Com; reflexivity
+  ]).
+Qed.
+
+(* used *)
+Lemma string_to_term__pair_append__commute : ∀ s s',
+  string_to_ka_term (pair_append s s') ≡ (string_to_ka_term s) ⋅ (string_to_ka_term s').
+Proof.
+  intros.
+  destruct s as (s1, s1'), s' as (s2, s2').
+  induction s1 as [|c1 s1 IHs1].
+  - induction s1' as [|c1' s1' IHs1'].
+    + simpl. repeat (rewrite Dot_Id2); reflexivity.
+    + simpl in *.
+      rewrite Dot_Assoc.
+      rewrite build_term__commutes; try (left; auto).
+      rewrite - Dot_Assoc.
+      rewrite IHs1'.
+      repeat (rewrite Dot_Id2).
+      repeat (rewrite Dot_Assoc).
+      reflexivity.
+  - simpl in *.
+    rewrite - Dot_Assoc.
+    rewrite IHs1.
+    repeat (rewrite Dot_Assoc).
+    reflexivity.
+Qed.
+
+(* unused *)
+Lemma destruct_power : ∀ t n s,
+  ka_pred_power (lang_interp t) n s ->
+    ∃ (ls : list (list T * list T)),
+      s = fold_right pair_append ([], []) ls
+        ∧ fold_right and True (List.map (lang_interp t) ls).
+Proof.
+  intros.
+  generalize dependent s.
+  induction n as [|n IHn].
+  - intros. simpl in H. unfold ka_pred_unit in H.
+    subst.
+    exists [].
+    simpl. repeat split.
+  - intros. simpl in H; unfold ka_pred_mul in H.
+    destruct H as [s1 [s2 [Hs1s2 [HLI1 Hpow]]]].
+    apply IHn in Hpow as [ls [Hs2 Hls]].
+    exists (s1::ls).
+    repeat split; try assumption.
+    simpl. rewrite - Hs2. assumption.
+Qed.
+
+(* used, but unused *)
+Lemma term_leq_term_star : ∀ (t : ka_term T), t ≤ t✶.
+Proof.
+  intros.
+  (* rewrite {2} Star. *)
+  rewrite Star.
+  rewrite Star.
+  rewrite Dist_L.
+  rewrite Dot_Id1.
+  rewrite Plus_Com.
+  rewrite - Plus_Assoc.
+  apply leq_plus.
+Qed.
+
+(* unused *)
+Lemma leq_term__leq_term_star : ∀ (t t': ka_term T), t ≤ t' -> t ≤ t'✶.
+Proof.
+  intros.
+  apply leq_trans with (t2:=t'); [assumption | apply term_leq_term_star].
+Qed.
+
+Lemma leq1__leq2__leq1_dot_2 : ∀ (t1 t2 t3 t4 : ka_term T),
+  t1 ≤ t3 -> t2 ≤ t4 -> t1⋅t2 ≤ t3⋅t4.
+Proof.
+  intros t1 t2 t3 t4 H1 H2.
+  unfold ka_leq in H1, H2.
+  rewrite - H1.
+  rewrite - H2.
+  rewrite Dist_R; repeat (rewrite Dist_L).
+  repeat (rewrite Plus_Assoc).
+  rewrite Plus_Com.
+  apply leq_plus.
+Qed.
+
+(* unused *)
+Lemma t__leq__t_star : ∀ (t : ka_term T), t ≤ t✶.
+Proof.
+  intros.
+  unfold ka_leq.
+  rewrite Star.
+  rewrite Star.
+  rewrite Dist_L.
+  rewrite Dot_Id1.
+  rewrite - Plus_Assoc.
+  assert (H : t + t ⋅ (t ⋅ t ✶) + t ≡ t + t ⋅ (t ⋅ t ✶) ).
+  { rewrite Plus_Com. rewrite Plus_Assoc.
+    rewrite Plus_Idemp. reflexivity. }
+  rewrite H.
+  rewrite Plus_Assoc.
+  reflexivity.
+Qed.
+
+(* used *)
+Lemma t_tstar__leq__tstar : ∀ (t : ka_term T), t⋅t✶ ≤ t✶.
+Proof.
+  intros.
+  rewrite [X in _ ≤ X] Star.
+  rewrite Plus_Com.
+  apply leq_plus.
+Qed.
+
+(* used, but unused *)
+Lemma leq__leq_dot_L : ∀ (t1 t2 t3 : ka_term T), t2 ≤ t3 -> t1 ⋅ t2 ≤ t1 ⋅ t3.
+Proof.
+  intros.
+  unfold ka_leq in H.
+  rewrite - H.
+  rewrite Dist_L.
+  rewrite Plus_Com.
+  apply leq_plus.
+Qed.
+
+(* unused *)
+Lemma leq__leq_dot_R : ∀ (t1 t2 t3 : ka_term T), t1 ≤ t3 -> t1 ⋅ t2 ≤ t3 ⋅ t2.
+Proof.
+  intros.
+  unfold ka_leq in H.
+  rewrite - H.
+  rewrite Dist_R.
+  rewrite Plus_Com.
+  apply leq_plus.
+Qed.
+
+(* unused *)
+Lemma pow_leq_star : ∀ (t : ka_term T) n, t^n ≤ t✶.
+Proof.
+  intros.
+  generalize dependent t.
+  induction n as [| n IHn].
+  - intros. unfold ka_power. apply one_leq_star.
+  - intros. simpl.
+    rewrite Star.
+    assert (H : t⋅t^n ≤ t⋅t✶).
+    { apply leq__leq_dot_L. apply IHn. }
+    apply leq_trans with (t2:=t⋅t✶).
+    + assumption.
+    + rewrite Plus_Com. apply leq_plus.
+Qed.
+
+(* Theorem 5 *)
+Theorem term_lang_equiv : ∀ s t, string_to_ka_term s ≤ t <-> lang_interp t s.
+Proof.
+  intros; split; intros H.
+  - unfold ka_leq in H.
+    rewrite l_i_equality. symmetry in H. apply H.
+    simpl.
+    unfold ka_pred_add. right.
+    apply li_term_to_string_true.
+  - generalize dependent s.
+    induction t; intros.
+    + simpl in H. contradiction.
+    + simpl in H. unfold ka_pred_unit in H.
+      subst. simpl. rewrite Dot_Id2. apply leq_reflex.
+    + inversion H. simpl. repeat (rewrite Dot_Id1). apply leq_reflex.
+    + inversion H. simpl. rewrite Dot_Id2; rewrite Dot_Id1; apply leq_reflex.
+    + simpl in H; unfold ka_pred_add in H. destruct H as [H1 | H2].
+      * apply IHt1 in H1.
+        apply leq_trans with (t2:=t1);
+        [assumption | apply leq_plus].
+      * apply IHt2 in H2.
+        apply leq_trans with (t2:=t2);
+        [assumption | rewrite Plus_Com; apply leq_plus].
+    + simpl in H. unfold ka_pred_mul in H.
+      destruct H as [s1 [s2 [Hs1s2 [HLI1 HLI2]]]].
+      apply IHt1 in HLI1; apply IHt2 in HLI2.
+      subst. destruct s1, s2. rewrite string_to_term__pair_append__commute.
+      apply leq_leq_dot; assumption.
+    + simpl in H. unfold ka_pred_star in H.
+      destruct H as [n H].
+      generalize dependent s.
+      induction n as [| n IHn].
+      * intros; simpl in H.
+        unfold ka_pred_unit in H; subst.
+        simpl; rewrite Dot_Id1.
+        apply one_leq_star.
+      * intros. simpl in H.
+        destruct H as [s1 [s2 [Hs1s2 [HLI1 Hpow]]]].
+        apply IHn in Hpow.
+        subst.
+        apply IHt in HLI1.
+        destruct s1 as (s1, s1'), s2 as (s2, s2').
+        rewrite string_to_term__pair_append__commute.
+        assert (H : string_to_ka_term (s1, s1') ⋅ string_to_ka_term (s2, s2') ≤ t⋅t✶).
+        {
+          apply leq1__leq2__leq1_dot_2; assumption.
+        }
+        apply leq_trans with (t2:=t⋅t✶);
+        [assumption | apply t_tstar__leq__tstar].
+Qed.
+
+(* unused *)
+Lemma zero_neq_one : (@K_Zero T ≢ @K_One T)%ka.
+Proof.
+  intros H.
+  (* QUEST: why was using apply not working here?? *)
+  have eq_langs := l_i_equality H.
+  specialize (eq_langs ([], [])).
+  simpl in eq_langs.
+  unfold ka_pred_zero, ka_pred_unit in eq_langs.
+  rewrite eq_langs.
+  reflexivity.
+Qed.
+
+(* unused *)
+Lemma zero_neq_L : ∀ a, (@K_Zero T ≢ L a).
+Proof.
+  intros a H.
+  have eq_langs := l_i_equality H.
+  specialize (eq_langs ([a], [])).
+  simpl in eq_langs.
+  unfold ka_pred_zero, ka_pred_left in eq_langs.
+  rewrite eq_langs.
+  reflexivity.
+Qed.
+
+(* unused *)
+Lemma zero_neq_R : ∀ a, (@K_Zero T ≢ R a).
+Proof.
+  intros a H.
+  have eq_langs := l_i_equality H.
+  specialize (eq_langs ([], [a])).
+  simpl in eq_langs.
+  unfold ka_pred_zero, ka_pred_left in eq_langs.
+  rewrite eq_langs.
+  reflexivity.
+Qed.
+
+(* unused *)
+Lemma zero_neq_one_plus_t : ∀ (t : ka_term T), 0 ≢ 1 + t.
+Proof.
+  intros t H.
+  have G := l_i_equality H.
+  specialize (G ([], [])).
+  simpl in G.
+  unfold ka_pred_zero, ka_pred_add, ka_pred_unit in G.
+  rewrite G. left. reflexivity.
+Qed.
+
+(* unused *)
+Lemma zero_neq_L_plus_t : ∀ (t : ka_term T) a, 0 ≢ L a + t.
+Proof.
+  intros t a H.
+  have G := l_i_equality H.
+  specialize (G ([a], [])).
+  simpl in G.
+  unfold ka_pred_zero, ka_pred_add, ka_pred_unit in G.
+  rewrite G. left. reflexivity.
+Qed.
+
+(* unused *)
+Lemma zero_neq_R_plus_t : ∀ (t : ka_term T) a, 0 ≢ R a + t.
+Proof.
+  intros t a H.
+  have G := l_i_equality H.
+  specialize (G ([], [a])).
+  simpl in G.
+  unfold ka_pred_zero, ka_pred_add, ka_pred_unit in G.
+  rewrite G. left. reflexivity.
+Qed.
+
+(* unused *)
+Lemma neq_reflex_false : ∀ (t : ka_term T), not (t ≢ t).
+Proof.
+  intros t H; apply H; reflexivity.
+Qed.
+
+(* Corollary 8' *)
+Lemma either_empty_or_nonzero : ∀ (t : ka_term T), t ≡ 0 ∨ ∃ s, lang_interp t s.
+Proof.
+  intros t.
+  induction t.
+  - left; reflexivity.
+  - right. exists ([], []). reflexivity.
+  - right. exists ([t], []). reflexivity.
+  - right. exists ([], [t]). reflexivity.
+  - destruct IHt1 as [IHt1 | IHt1]; destruct IHt2 as [IHt2 | IHt2].
+    + left. rewrite IHt1. rewrite IHt2. apply Plus_Idemp.
+    + right. destruct IHt2 as [s H].
+      exists s. rewrite IHt1.
+      rewrite Plus_Id; assumption.
+    + right; destruct IHt1 as [s H].
+      exists s; rewrite IHt2.
+      rewrite Plus_Id'.
+      assumption.
+    + destruct IHt1 as [s1 H1], IHt2 as [s2 H2].
+      right. exists s1.
+      simpl. unfold ka_pred_add.
+      left; assumption.
+  - destruct IHt1 as [H1 | H1]; destruct IHt2 as [H2 | H2].
+    + left. rewrite H1. apply Dot_Z2.
+    + left. rewrite H1. apply Dot_Z2.
+    + left. rewrite H2. apply Dot_Z1.
+    + destruct H1 as [s1 H1], H2 as [s2 H2].
+      right.
+      exists (pair_append s1 s2).
+      simpl.
+      unfold ka_pred_mul.
+      exists s1, s2.
+      auto.
+  - right. exists ([], []).
+    simpl.
+    unfold ka_pred_star.
+    exists 0%nat.
+    reflexivity.
+Qed.
 
 
+Lemma interp_build_term_l : ∀ s, lang_interp (build_term L 1 s) (s, []).
+Proof.
+  intros s. induction s as [| c s IHs].
+  - reflexivity.
+  - simpl in *.
+    unfold ka_pred_mul, ka_pred_left.
+    exists ([c], []), (s, []).
+    repeat split; intuition.
+Qed.
 
-  split; intros; simpl in *.
-    + destruct H as [s1 [s2 [Hs1s2 [HLI1 [s3 [s4 [Hs3s4 [HLI3 HLI4]]]]]]]].
-      exists s1, s2; repeat split.
-      destruct H as [s1 [s2 [Hs1s2 [HLI1 [s3 [s4 [Hs3s4 [HLI3 HLI4]]]]]]]].
+Lemma interp_build_term_r : ∀ s, lang_interp (build_term R 1 s) ([], s).
+Proof.
+  intros s. induction s as [| c s IHs].
+  - reflexivity.
+  - simpl in *.
+    unfold ka_pred_mul, ka_pred_left.
+    exists ([], [c]), ([], s).
+    repeat split; intuition.
+Qed.
 
+(* would be nice to prove *)
+(* Lemma test : ∀ (t t' : ka_term T), t ≤ t' -> t ≡ t' ∨ ∃ s, lang_interp t' s ∧ not (lang_interp t s).
+Proof.
+  intros.
+  unfold ka_leq in H.
+  have eq_langs := l_i_equality H.
+  simpl in eq_langs.
+  unfold ka_pred_add in eq_langs.
+  left. *)
 
-Fixpoint R_M' (P : list mm2_instr) (n : nat) := match P with
-  | [] => 0
-  | hd :: tl => (interp 1 P) ⋅ (L (Q_M n)) + R_M' tl (S n)
+(* Corollary 8'' *)
+Lemma no_string_leq_0 : ∀ s, not (string_to_ka_term s ≤ 0).
+Proof.
+  intros s H.
+  unfold ka_leq in H.
+  rewrite Plus_Id in H.
+  destruct s as (s1, s2).
+  simpl in H.
+  have eq_langs := l_i_equality H.
+  specialize (eq_langs (s1, s2)).
+  simpl in eq_langs; unfold ka_pred_mul, ka_pred_zero in eq_langs.
+  apply eq_langs.
+  exists (s1, []), ([], s2).
+  repeat split.
+  - simpl; rewrite app_nil_r; reflexivity.
+  - apply interp_build_term_l.
+  - apply interp_build_term_r.
+Qed.
+
+(* unused *)
+Lemma no_string_equiv_0 : ∀ s, string_to_ka_term s ≢ 0.
+Proof.
+  intros s H.
+  rewrite <- Plus_Id in H. (* QUEST: ssreflect way of writing this? *)
+  apply no_string_leq_0 in H; assumption.
+Qed.
+
+(* unused *)
+Lemma zero_leq_anything : ∀ (t : ka_term T), 0 ≤ t.
+Proof.
+  intros.
+  unfold ka_leq.
+  apply Plus_Id'.
+Qed.
+
+Lemma zero_eq_sum : ∀ (t t' : ka_term T), 0 ≡ t + t' <-> 0 ≡ t ∧ 0 ≡ t'.
+Proof.
+  intros t t'; split.
+  - intros H. generalize dependent t'.
+    induction t.
+    + intros t' H. rewrite Plus_Id in H.
+      intuition.
+    + intros t' H.
+      apply zero_neq_one_plus_t in H.
+      exfalso; assumption.
+    + intros t' H.
+      apply zero_neq_L_plus_t in H.
+      exfalso; assumption.
+    + intros t' H.
+      apply zero_neq_R_plus_t in H.
+      exfalso; assumption.
+    + intros t' H.
+      rewrite - Plus_Assoc in H.
+      apply IHt1 in H as [H1 H2].
+      apply IHt2 in H2 as [H2 H3].
+      rewrite - H1.
+      rewrite - H2.
+      rewrite Plus_Idemp.
+      intuition.
+    + intros t' H.
+    admit.
+    + intros t' H.
+      rewrite Star in H.
+      rewrite - Plus_Assoc in H.
+      apply zero_neq_one_plus_t in H.
+      contradiction.
+  - intros [H1 H2].
+    rewrite - H1; rewrite - H2.
+    rewrite Plus_Id.
+    reflexivity.
+Admitted.
+
+Lemma zero_eq_prod : ∀ (t1 t2 : ka_term T), 0 ≡ t1 ⋅ t2 -> t1 ≡ 0 ∨ t2 ≡ 0.
+Proof.
+  intros t1 t2 H.
+  generalize dependent t2.
+  induction t1.
+  - intros t2 H; left; reflexivity.
+  - intros t2 H. rewrite Dot_Id2 in H.
+    right; symmetry; assumption.
+  - intros t2 H.
+    have [Ht2 | [s Ht2]] := either_empty_or_nonzero t2.
+    + right; assumption.
+    + have eq_langs := l_i_equality H.
+      simpl in eq_langs.
+      unfold ka_pred_zero, ka_pred_mul, ka_pred_left in eq_langs.
+      exfalso; rewrite eq_langs.
+      exists ([t], []), s.
+      repeat split.
+      auto.
+  - intros t2 H.
+    have [Ht2 | [s Ht2]] := either_empty_or_nonzero t2.
+    + right; assumption.
+    + have eq_langs := l_i_equality H.
+      simpl in eq_langs.
+      unfold ka_pred_zero, ka_pred_mul, ka_pred_right in eq_langs.
+      exfalso; rewrite eq_langs.
+      exists ([], [t]), s.
+      repeat split.
+      auto.
+  - intros t2 H.
+    Search K_Zero.
+    have [Ht2 | [s Ht2]] := either_empty_or_nonzero t2.
+    + right; assumption.
+    + have eq_langs := l_i_equality H.
+      simpl in eq_langs.
+      unfold ka_pred_zero, ka_pred_mul, ka_pred_add in eq_langs.
+Admitted.
+
+(* used but unused *)
+Lemma zero_neq_prod : ∀ (t1 t2 : ka_term T), 0 ≢ t1 ⋅ t2 (*<*)-> t1 ≢ 0 ∧ t2 ≢ 0.
+Proof.
+  (* split;  *)intros t1 t2 H.
+  split; intros G.
+    + rewrite G in H.
+      rewrite Dot_Z2 in H.
+      apply H; reflexivity.
+    + rewrite G in H.
+      rewrite Dot_Z1 in H.
+      apply H; reflexivity.
+Qed.
+
+(* unused *)
+Lemma zero_neq_const_dot_term : ∀ (t t': ka_term T) a, (t ≡ 1 ∨ t ≡ L a ∨ t ≡ R a) -> 0 ≢ t⋅t' -> 0 ≢ t'.
+Proof.
+  intros t t' a H G.
+  destruct H as [H | [H | H]]; rewrite H in G; clear H;
+  try (rewrite Dot_Id2 in G; assumption);
+  apply zero_neq_prod in G as [G1 G2];
+  apply ka_neq_sym; assumption.
+Qed.
+
+(* QUEST: is there a nice way to merge these two lemmas? *)
+Lemma lang_interp_build_l : ∀ (s1 s2 s3 : list T),
+  lang_interp (build_term L 1 s1) (s2, s3) -> s2 = s1 ∧ s3 = [].
+Proof.
+  intros s1 s2 s3 H. simpl in H.
+  generalize dependent s2;
+  generalize dependent s3.
+  induction s1 as [|c s1 IHs1].
+  + intros. simpl in H; unfold ka_pred_unit in H.
+    inversion H. intuition.
+  + intros.
+    simpl in H;
+    unfold ka_pred_mul in H.
+    destruct H as [s4 [s5 [Hp [Hl HLI]]]].
+    unfold ka_pred_left in Hl.
+    subst. destruct s5 as (s5, s5'). simpl in Hp.
+    inversion Hp; subst.
+    apply IHs1 in HLI as [Heq H5].
+    subst. intuition.
+Qed.
+
+Lemma lang_interp_build_r : ∀ (s1 s2 s3 : list T),
+  lang_interp (build_term R 1 s1) (s2, s3) -> s1 = s3 ∧ s2 = [].
+Proof.
+  intros s1 s2 s3 H. simpl in H.
+  generalize dependent s2;
+  generalize dependent s3.
+  induction s1 as [|c s1 IHs1].
+  + intros. simpl in H; unfold ka_pred_unit in H.
+    inversion H. intuition.
+  + intros.
+    simpl in H;
+    unfold ka_pred_mul in H.
+    destruct H as [s4 [s5 [Hp [Hr HLI]]]].
+    unfold ka_pred_right in Hr.
+    subst. destruct s5 as (s5, s5'). simpl in Hp.
+    inversion Hp. subst.
+    apply IHs1 in HLI as [Heq H5].
+    subst. intuition.
+Qed.
+
+Lemma string_interp_self : ∀ s s', lang_interp (string_to_ka_term s) s' <-> s = s'.
+Proof.
+  intros.
+  split.
+  - intros H.
+    destruct s as (s1, s2), s' as (s1', s2').
+    simpl in H.
+    unfold ka_pred_mul in H.
+    destruct H as [s3 [s4 [Hs1s2' [HLIs1 HLIs2]]]].
+    destruct s3 as (s3, s3'), s4 as (s4, s4').
+    simpl in Hs1s2'.
+    rewrite Hs1s2'.
+    apply lang_interp_build_l in HLIs1 as [H1 H2];
+    apply lang_interp_build_r in HLIs2 as [H3 H4].
+    subst; simpl; rewrite app_nil_r.
+    reflexivity.
+  - intros H. rewrite H.
+    apply li_term_to_string_true.
+Qed.
+
+Fixpoint map_indexed' {A} {B} (f : nat -> A -> B) n ls :=
+  match ls with
+  | [] => []
+  | hd :: tl => f n hd :: map_indexed' f (S n) tl
   end.
 
-Definition R_M (P : list mm2_instr) := R_M' P 1.
+Definition map_indexed {A} {B} (f : nat -> A -> B) ls := map_indexed' f 0 ls.
 
-Fixpoint C_M' (P : list mm2_instr) (n : nat) := match P with
+Definition term_product (ls : list (ka_term T)) := fold_right (λ t t', t⋅t') 1 ls.
+
+Definition term_sum (ls : list (ka_term T)) := fold_right (λ t t', t+t') 0 ls.
+
+Definition cstring_sum (ls : list (list T * list T)) := term_sum (map string_to_ka_term ls).
+
+Definition finite_term t := ∃ ls, ∀ s, In s ls <-> lang_interp t s.
+
+(* Lemma test : ∀ (P Q R : (list T * list T) -> Prop), (∀ s, P s <-> Q s) -> (∀ s, P s <-> Q s ∨ R s).
+Proof.
+  intros. *)
+
+Lemma finite_terms__finite_sum : ∀ t t', finite_term t ∧ finite_term t' -> finite_term (t + t').
+Proof.
+  intros t t' [[l1 H1] [l2 H2]].
+  unfold finite_term.
+  simpl.
+  unfold ka_pred_add.
+  exists (l1 ++ l2).
+  intros s.
+  split.
+  + intros H.
+    apply in_app_or in H as [H | H];
+    [apply H1 in H | apply H2 in H];
+    intuition.
+  + intros [H | H]; apply in_or_app;
+    [apply H1 in H | apply H2 in H];
+    intuition.
+Qed.
+
+Lemma finite_term_dist_over_plus : ∀ t t', finite_term (t + t') <-> finite_term t ∧ finite_term t'.
+Proof.
+  intros t t'. split.
+  - intros [ls H].
+    simpl in H;
+    unfold ka_pred_add in H.
+    (* admit. *)
+    split; unfold finite_term.
+    + exists ls.
+      intros s.
+      rewrite H.
+      split.
+      * intros [G | G]; try assumption.
+        admit.
+      * intuition.
+    + exists ls.
+      intros s.
+      rewrite H.
+      split.
+      * intros [G | G]; try assumption.
+        admit.
+      * intuition.
+  - intros [[l1 H1] [l2 H2]].
+    unfold finite_term.
+    simpl.
+    unfold ka_pred_add.
+    exists (l1 ++ l2).
+    intros s.
+    split.
+    + intros H.
+      apply in_app_or in H as [H | H];
+      [apply H1 in H | apply H2 in H];
+      intuition.
+    + intros [H | H]; apply in_or_app;
+      [apply H1 in H | apply H2 in H];
+      intuition.
+Admitted.
+
+Lemma finite_term_dist_over_dot : ∀ t t', finite_term (t ⋅ t') <-> finite_term t ∧ finite_term t'.
+Proof.
+Admitted.
+
+Lemma cstring_app_commute : ∀ l1 l2,
+  cstring_sum (l1 ++ l2) ≡ (cstring_sum l1) + (cstring_sum l2).
+Proof.
+  intros.
+  induction l1 as [| c1 l1 IHl1].
+  + simpl.
+    unfold cstring_sum; simpl.
+    rewrite Plus_Id; reflexivity.
+  + simpl. unfold cstring_sum. simpl.
+    unfold cstring_sum in IHl1.
+    rewrite IHl1.
+    apply Plus_Assoc.
+Qed.
+
+(* Theorem 6' *)
+Theorem finite_def : ∀ t,
+  (∃ ls, t ≡ cstring_sum ls)
+  <->
+  finite_term t.
+Proof.
+  intros t; split.
+  - intros [ls H].
+    exists ls.
+    intros s.
+    rewrite H; clear H.
+    induction ls as [| c ls IHls].
+    + simpl. reflexivity.
+    + simpl. unfold ka_pred_add.
+      rewrite - IHls.
+      rewrite string_interp_self.
+      reflexivity.
+  -
+    (* intros [ls H].
+    exists ls.
+    induction t.
+    + simpl in H. unfold ka_pred_zero in H.
+      induction ls.
+      * reflexivity.
+      * specialize (H a0). simpl in H.
+        exfalso; apply H. intuition.
+    + simpl in H. unfold ka_pred_unit in H.
+      induction ls as [| c ls IHls].
+      * specialize (H ([], []));
+        simpl in H.
+        exfalso; intuition.
+      * simpl in H.
+        specialize (H c); simpl in H. *)
+    (* unfold finite_term. *)
+    (* intros [ls H]. *)
+    induction t(* ; intros [ls H] *).
+    + intros [ls H]. exists []. reflexivity.
+    + intros [ls H]. exists [([], [])]. unfold cstring_sum. simpl.
+      rewrite Dot_Id2; rewrite Plus_Id'.
+      reflexivity.
+    + intros [ls H]. exists [([t], [])]; unfold cstring_sum; simpl.
+      repeat (rewrite Dot_Id1);
+      rewrite Plus_Id'.
+      reflexivity.
+    + intros [ls H]. exists [([], [t])]; unfold cstring_sum; simpl.
+      rewrite Dot_Id1;
+      rewrite Dot_Id2;
+      rewrite Plus_Id'.
+      reflexivity.
+    + rewrite finite_term_dist_over_plus. intros [H1 H2].
+      apply IHt1 in H1 as [l1 H1].
+      apply IHt2 in H2 as [l2 H2].
+      exists (l1 ++ l2).
+      simpl.
+      rewrite cstring_app_commute.
+      rewrite H1; rewrite H2.
+      reflexivity.
+    (* + rewrite finite_term_dist_over_dot. intros [H1 H2].
+      apply IHt1 in H1 as [l1 H1].
+      apply IHt2 in H2 as [l2 H2].
+
+    intros [[l1 H1] [l2 H2]]. simpl in H.
+      unfold ka_pred_add in H.
+      unfold finite_term in IHt1, IHt2.
+      induction ls as [|c ls IHls].
+      * have [t_cond1 | [s1 t_cond1]] := either_empty_or_nonzero t1;
+        have [t_cond2 | [s2 t_cond2]] := either_empty_or_nonzero t2;
+        try (specialize (H s1); simpl in H; exfalso; rewrite H; intuition).
+        -- exists []. rewrite t_cond1; rewrite t_cond2; rewrite Plus_Idemp.
+           reflexivity.
+        -- specialize (H s2).
+           simpl in H.
+           exfalso. rewrite H. intuition.
+      * simpl in H.
+        specialize (H c) as [c' H]. *)
+Admitted.
+
+(* Corollary 7' *)
+Theorem finite_terms_interp__equiv : ∀ (t t' : ka_term T),
+  finite_term t -> finite_term t' ->
+    (∀ s, lang_interp t s <-> lang_interp t' s) ->
+      t ≡ t'.
+Proof.
+  intros t t' Hft Hft' Hli.
+  have Hft1 := Hft.
+  have Hft1' := Hft'.
+  apply finite_def in Hft1 as [ls Htsum], Hft1' as [ls' Htsum'].
+  destruct Hft as [s Ht], Hft' as [s' Ht'].
+  rewrite Htsum.
+  rewrite Htsum'.
+  unfold cstring_sum.
+  unfold cstring_sum.
+  induction ls as [|c ls IHls], ls' as [|c' ls'].
+  - reflexivity.
+  - simpl in *.
+    unfold cstring_sum in Htsum.
+    simpl in Htsum.
+  induction ls as [|c ls IHls].
+  - unfold cstring_sum in Htsum. simpl in Htsum. simpl.
+  assert (G : cstring_sum ls ≡ cstring_sum ls').
+  {
+    unfold cstring_sum.
+    unfold map.
+    compute.
+  }
+
+(* QUEST: How to allow term_list_to_term to be generic here? *)
+
+(* Definition C_M (P : list mm2_instr) := *)
+
+
+
+(* Fixpoint R_M' (P' P : list mm2_instr) (n : nat) := match P with
+  | [] => 0
+  | hd :: tl => (interp n P) ⋅ (L (Q_M n)) + R_M' tl P (S n)
+  end. *)
+
+(* Definition R_M (P : list mm2_instr) := R_M' P P 1. *)
+
+(* Fixpoint C_M' (P : list mm2_instr) (n : nat) := match P with
   | [] => 0
   | _::tl => L (Q_M n) + C_M' tl (S n)
-  end.
+  end. *)
 
-Definition C_M (P : list mm2_instr) := (L a)✶ ⋅ (L b)✶ ⋅ (C_M' P 1).
+(* Definition C_M (P : list mm2_instr) := (L a)✶ ⋅ (L b)✶ ⋅ (C_M' P 1). *)
 
 End Theory.
-Local Open Scope ka_scope.
+(* -------------- *)
 
-Check string_to_ka_term.
-Theorem R_M__well_formed : ∀ P (s s' : list Σ_M), step Σ_M s s' (R_M P) -> (string_to_ka_term Σ_M L s ≤ C_M P).
+Definition R_M (P : list mm2_instr) :=
+   term_list_to_term (map_indexed interp_single P).
+
+(* Local Open Scope ka_scope. *)
+
+Example string_to_ka_term__test1 :
+  string_to_ka_term ([a; b; a; a], [a; b; a; a]) ≡ (lr a ⋅ lr b ⋅ lr a ⋅ lr a).
 Proof.
-  intros. unfold step in H. unfold string_to_ka_term in *. unfold C_M. unfold ka_leq. compute.
+  simpl; unfold lr_term.
+  rewrite Dot_Id1.
+  repeat (rewrite Dot_Assoc).
+  reflexivity.
+Qed.
 
-Definition lang_interp {T} (term : ka_term T) :=
-  match term with
-  | L x => ([x], [])
-  | R x => ([], [x])
-  | K_Plus x y => ([], [])
-  | _ => ([], [])
-  end.
+Example string_to_ka_term__test2 :
+  string_to_ka_term Σ_M [a; b; c_1] ≡ lr a ⋅ lr b ⋅ lr c_1.
+Proof.
+  simpl; unfold lr_term.
+  rewrite Dot_Id1.
+  repeat (rewrite Dot_Assoc).
+  reflexivity.
+Qed.
+
 Check lang_interp.
-
-Print mm2_instr.
-Search mm2_atom.
-Print mm2_step.
-(* Definition mm2_instr__to__katerm instr := match
-  instr with
-  | mm2_inc_a => (R a) ⋅ (lr a)✶ ⋅ (lr b)✶
-  | _ => R a
-  end
-. *)
+Theorem term_leq_R_M__in_lang_interp : ∀ P s s', (string_to_ka_term Σ_M L s) ⋅ (string_to_ka_term Σ_M R s') ≤ R_M P <-> lang_interp Σ_M (R_M P) (s, s').
+Proof.
+  simpl; split; intros.
+  - unfold R_M.
 
 Fixpoint to_term (f : T -> ka_term T) (s : list T) :=
   match s with
@@ -659,10 +1422,10 @@ Fixpoint left_assoc e :=
   | t => t
   end.
 
-(* Theorem left_assoc_equiv e : left_assoc e ≐ e.
+(* Theorem left_assoc_equiv e : left_assoc e ≡ e.
 Proof.
   induction e; try (reflexivity).
-  - assert (H : left_assoc (e1 + e2) ≐ (left_assoc e1) + left_assoc e2).
+  - assert (H : left_assoc (e1 + e2) ≡ (left_assoc e1) + left_assoc e2).
     { simpl. inversion IHe2; subst. compute. }
   rewrite <- IHe1. generalize dependent IHe2.
     induction e2; try reflexivity.
@@ -672,13 +1435,13 @@ Proof.
 
 (* Definition canonicalize e := left_assoc (remove_1 (compose_L_R (collect_L_R e [] []))).
 
-Theorem canonicalize_equiv e : canonicalize e ≐ e.
+Theorem canonicalize_equiv e : canonicalize e ≡ e.
 Proof.
   induction e; try (compute; reflexivity).
   - unfold canonicalize.
     assert
     unfold collect_L_R.
-  assert (H : canonicalize (e1 + e2) ≐ (canonicalize e1) + (canonicalize e2)).
+  assert (H : canonicalize (e1 + e2) ≡ (canonicalize e1) + (canonicalize e2)).
     { rewrite IHe1. rewrite IHe2. compute. }
   unfold canonicalize.
     unfold collect_L_R. *)
@@ -687,7 +1450,7 @@ End Canonicalization.
 
 Local Open Scope ka_scope.
 
-Example check_canonicalize : canonicalize Σ_M (R a ⋅ L a ⋅ R b ⋅ L b) ≐ L a ⋅ L b ⋅ R a ⋅ R b.
+Example check_canonicalize : canonicalize Σ_M (R a ⋅ L a ⋅ R b ⋅ L b) ≡ L a ⋅ L b ⋅ R a ⋅ R b.
 Proof.
   (* simpl. why does simpl not do anything here? compute does more *)
   compute. reflexivity.
@@ -709,28 +1472,28 @@ Theorem canonicalize_equiv :
   | s => s
   end. *)
 
-(* Example to_L__R_ex1 : ∀ x y, to_L__R ((lr x)⋅(lr y)) ≐ (L x)⋅(L y)⋅(R x)⋅(R y).
+(* Example to_L__R_ex1 : ∀ x y, to_L__R ((lr x)⋅(lr y)) ≡ (L x)⋅(L y)⋅(R x)⋅(R y).
 Proof.
   intros.
   (* unfold lr_term. *)
   reflexivity.
 Qed.
 
-Example to_L__R_ex2 : ∀ x y z, to_L__R ((lr x)⋅(lr y)⋅(lr z)) ≐ L x⋅L y⋅L z⋅R x⋅R y⋅R z.
+Example to_L__R_ex2 : ∀ x y z, to_L__R ((lr x)⋅(lr y)⋅(lr z)) ≡ L x⋅L y⋅L z⋅R x⋅R y⋅R z.
 Proof.
   intros.
   simpl. *)
 
 
 
-Lemma plus_interleave : ∀ (x y z w : ka_term T), x + y + z + w ≐ x + z + y + w.
+Lemma plus_interleave : ∀ (x y z w : ka_term T), x + y + z + w ≡ x + z + y + w.
 Proof.
   intros.
   rewrite <- Plus_Assoc.
   rewrite <- Plus_Assoc.
-  assert (G : y + (z + w) ≐ (z + w) + y). { apply Plus_Com. }
+  assert (G : y + (z + w) ≡ (z + w) + y). { apply Plus_Com. }
   rewrite G.
-  assert (H : y + w ≐ w + y). { apply Plus_Com. }
+  assert (H : y + w ≡ w + y). { apply Plus_Com. }
   rewrite <- Plus_Assoc.
   rewrite <- H.
   rewrite Plus_Assoc.
@@ -738,7 +1501,7 @@ Proof.
   reflexivity.
 Qed.
 
-Lemma extra_one_ignore : forall (x : ka_term T), 1 + 1 + x ≐ 1 + x.
+Lemma extra_one_ignore : forall (x : ka_term T), 1 + 1 + x ≡ 1 + x.
 Proof.
   intros.
   rewrite Plus_Idemp.
@@ -751,7 +1514,7 @@ Locate "lr".
 
 
 
-Lemma x_xstar__xtar_x : forall (t : ka_term T), t⋅t✶ ≐ t✶⋅t.
+Lemma x_xstar__xtar_x : forall (t : ka_term T), t⋅t✶ ≡ t✶⋅t.
 Proof.
   intros.
   induction t.
@@ -760,10 +1523,10 @@ Proof.
   - admit.
   - admit.
   - rewrite Dist_R. rewrite Dist_L.
-Admitted. (* should follow from t⋅t✶ ≐ t✶ ≐ t✶⋅t *)
+Admitted. (* should follow from t⋅t✶ ≡ t✶ ≡ t✶⋅t *)
 
 
-Lemma x_x_star : forall (t : ka_term T), t✶ ≐ t✶⋅t.
+Lemma x_x_star : forall (t : ka_term T), t✶ ≡ t✶⋅t.
 Proof.
   intros.
   assert (H : t✶ ≤ t✶⋅t).
@@ -783,7 +1546,7 @@ Admitted.
   rewrite Dot_Id1.
   rewrite Dot_Assoc.
   rewrite <- star_expand.
-  assert (H : t ≐ t⋅1).
+  assert (H : t ≡ t⋅1).
   { symmetry. apply Dot_Id1. }
   rewrite <- Dot_Assoc.
   rewrite H.
@@ -817,7 +1580,7 @@ Print ka_term.
 Check term_to_disjoint_term ([[a]]⋅[[b]]⋅[[Q_M 1]]). *)
 (* Example ex_1 :
   term_to_disjoint_term ([[a]]⋅[[b]]⋅[[Q_M 1]])
-  ≐ [[l a]]⋅[[r a]]⋅[[l b]]⋅[[r b]]⋅[[l (Q_M 1)]]⋅[[r (Q_M 1)]].
+  ≡ [[l a]]⋅[[r a]]⋅[[l b]]⋅[[r b]]⋅[[l (Q_M 1)]]⋅[[r (Q_M 1)]].
   Proof. simpl. Unset Printing Notations. *)
 
 
@@ -857,7 +1620,7 @@ Proof.
 Qed.
 
 Lemma ka_power_decomp : forall T (kat : ka_term T) n m,
-  ka_power kat (n + m) ≐ K_Dot (ka_power kat n) (ka_power kat m).
+  ka_power kat (n + m) ≡ K_Dot (ka_power kat n) (ka_power kat m).
 Proof.
   intros.
   induction n.
@@ -865,20 +1628,20 @@ Proof.
   - simpl. rewrite IHn. rewrite Dot_Assoc. reflexivity.
 Qed.
 
-Lemma test : forall T (t : ka_term T), t + 0 ≐ t.
+Lemma test : forall T (t : ka_term T), t + 0 ≡ t.
 Proof.
 intros. rewrite Plus_Com. by constructor. Qed.
 
 Lemma plus_assoc_swap1 : ∀ T (x y z : ka_term T),
-  x + (y + z) ≐ x + (z + y).
+  x + (y + z) ≡ x + (z + y).
 Proof.
-  intros. assert (H: y+z ≐ z + y).
+  intros. assert (H: y+z ≡ z + y).
   - apply Plus_Com.
   - rewrite H. reflexivity.
 Qed.
 
 Lemma plus_assoc_swap2 : ∀ T (x y z : ka_term T),
-  x + (y + z) ≐ (x + z) + y.
+  x + (y + z) ≡ (x + z) + y.
 Proof.
   intros. assert (H: y+z≐z+y).
   - apply Plus_Com.
@@ -886,16 +1649,9 @@ Proof.
 Qed.
 
 (* QUEST: why does this struggle with typing? *)
-Lemma test_1 : forall (T:Type) (x y z : ka_term T), x ≤ y -> (x + z ≐ (x + y) + z).
+Lemma test_1 : forall (T:Type) (x y z : ka_term T), x ≤ y -> (x + z ≡ (x + y) + z).
 Proof.
   intros. unfold ka_leq in H. rewrite Plus_Com in H. rewrite H. reflexivity.
-Qed.
-
-Lemma leq_antisym : forall (T : Type) (x y : ka_term T), x ≤ y -> y ≤ x -> x ≐ y.
-Proof.
-  intros.
-  unfold ka_leq in H, H0.
-  rewrite <- H. rewrite Plus_Com. assumption.
 Qed.
 
 Global Instance leq_trans : ∀ T, Transitive (@ka_eq T).
